Proof for generic Call<Function>
There's some trouble with the function name possibly shadowing the local
variable names

src/program_proof/lockservice/common_proof.v
@@ -1,4 +1,4 @@
-From Perennial.program_proof.lockservice Require Import lockservice fmcounter_map nondet.
+From Perennial.program_proof.lockservice Require Import lockservice fmcounter_map nondet rpc.
 From iris.program_logic Require Export weakestpre.
 From Perennial.goose_lang Require Import prelude.
 From Perennial.goose_lang Require Import ffi.disk_prelude.
@@ -67,4 +67,93 @@ Proof.
     by iApply "Hpost".
   }
 Qed.
+
+(* Returns true iff server reported error or request "timed out" *)
+Definition CallFunction (f:val) (fname:string) (rty_desc:descriptor) : val :=
+  rec: "" "srv" "args" "reply" :=
+    Fork (let: "dummy_reply" := struct.alloc rty_desc (zero_val (struct.t rty_desc)) in
+          Skip;;
+          (for: (λ: <>, #true); (λ: <>, Skip) := λ: <>,
+            f "srv" "args" "dummy_reply";;
+            Continue));;
+    (if: nondet #()
+    then f "srv" "args" "reply"
+    else #true).
+
+Lemma CallFunction_spec {A:Type} {R:Type} {a_req:RPCRequest A} (srv args reply:loc) (lockArgs:A) (lockReply:R) (f:val) (fname:string) (rty_desc:descriptor) fPre fPost γrpc γPost {r_rpc: RPCReply R rty_desc} :
+has_zero (struct.t rty_desc)
+-> (∀ srv' args' lockArgs' γrpc' γPost', Persistent (fPre srv' args' lockArgs' γrpc' γPost'))
+-> (∀ (srv' args' reply' : loc) (lockArgs':A) 
+   (lockReply' : R) (γrpc' : RPC_GS) (γPost' : gname),
+{{{ fPre srv' args' lockArgs' γrpc' γPost'
+    ∗ own_reply reply' lockReply'
+}}}
+  f #srv' #args' #reply'
+{{{ RET #false; ∃ lockReply',
+    own_reply reply' lockReply'
+    ∗ fPost lockArgs' lockReply' γrpc'
+}}}
+)
+      ->
+{{{ "#HfPre" ∷ fPre srv args lockArgs γrpc γPost ∗ "Hreply" ∷ own_reply reply lockReply }}}
+  (CallFunction f fname rty_desc) #srv #args #reply
+{{{ e, RET e;
+    (∃ lockReply',
+    own_reply reply lockReply'
+        ∗ (⌜e = #true⌝ ∨ ⌜e = #false⌝ ∗ fPost lockArgs lockReply' γrpc))
+}}}.
+Proof.
+  intros Hhas_zero Hpers Hspec.
+  iIntros (Φ) "Hpre Hpost".
+  iNamed "Hpre".
+  wp_lam.
+  wp_let.
+  wp_let.
+  wp_apply wp_fork.
+  {
+    wp_apply (wp_allocStruct); first eauto.
+    iIntros (l) "Hl".
+    iDestruct (alloc_reply with "Hl") as "Hreply".
+    wp_let. wp_pures.
+    wp_apply (wp_forBreak
+                (fun b => ⌜b = true⌝∗
+                                   ∃ reply, (own_reply l reply)
+                )%I with "[] [Hreply]");
+             try eauto.
+
+    iIntros (Ψ).
+    iModIntro.
+    iIntros "[_ Hpre] Hpost".
+    iDestruct "Hpre" as (reply') "Hreply".
+    wp_apply (Hspec with "[Hreply]"); eauto; try iFrame "#".
+
+    iIntros "fPost".
+    wp_seq.
+    iApply "Hpost".
+    iSplitL ""; first done.
+    iDestruct "fPost" as (reply'') "[Hreply fPost]".
+    iExists _. iFrame.
+  }
+  wp_seq.
+  wp_apply (nondet_spec).
+  iIntros (choice) "[Hv|Hv]"; iDestruct "Hv" as %->.
+  {
+    wp_pures.
+    wp_apply (Hspec with "[$Hreply]"); eauto; try iFrame "#".
+    iDestruct 1 as (reply') "[Hreply fPost]".
+    iApply "Hpost".
+    iFrame.
+    iExists _; iFrame.
+    iRight.
+    iSplitL ""; first done.
+    iFrame.
+  }
+  {
+    wp_pures.
+    iApply "Hpost".
+    iExists _; iFrame "Hreply".
+    by iLeft.
+  }
+Qed.
+
 End lockservice_common_proof.
